code/rsapss/Hacl.Bignum4096.fst
@@ -85,3 +85,5 @@ let mod_exp =
 let new_bn_from_bytes_be = Hacl.Bignum.Convert.new_bn_from_bytes_be
 
 let bn_to_bytes_be = Hacl.Bignum.Convert.mk_bn_to_bytes_be n
+
+let lt = Hacl.Bignum.mk_bn_is_less n
