Makefile
@@ -640,6 +640,7 @@ INTRINSIC_FLAGS = -add-include '"libintvector.h"'
 # Disabled for distributions that don't include code based on intrinsics.
 INTRINSIC_INT_FLAGS = \
   -add-include 'Hacl_ECDSA:"lib_intrinsics.h"' \
+  -add-include 'Hacl_Bignum4096:"lib_intrinsics.h"' \
   -add-include 'Hacl_RSAPSS:"lib_intrinsics.h"'
 
 # Disabled for dist/portable
